imp_compile/ImpSimple.v
@@ -22,6 +22,7 @@ Section Example_Extract.
   |}.
 
   Definition imp_simple_prog : program := {|
+    name := "Simple";
     ext_vars := [];
     ext_funs := [];
     prog_vars := [];
